rewrite Minimalistic.v
- use PositiveMap instead of list bool for randomness
- define (but do not prove equivalence) of alternative interpretation
  function
- use [Comp_eq] whenever possible
- significantly shorter the proofs of all proven lemmas

cc @abergal

Ready for try #1 on encryption?

- https://eprint.iacr.org/2016/069.pdf section 11.1
- "A Computationally Complete Symbolic Attacker for Equivalence Properties" section 7 page 617 left bottom

src/Minimalistic.v
@@ -12,414 +12,177 @@ Require Import Util.
 Require Import Coq.Classes.Morphisms.
 Require Import Coq.Lists.SetoidList.
 Require Import Coq.Lists.ListSet.
+Require Import Coq.MSets.MSetPositive.
+Require Import Coq.FSets.FMapPositive.
+Require Import Coq.FSets.FMapFacts.
+Module PositiveMapFacts := FMapFacts.WFacts_fun PositiveMap.E PositiveMap.
+Module PositiveMapProperties := FMapFacts.WProperties_fun PositiveMap.E PositiveMap.
+
+Lemma Bind_unused A B (a:Comp A) (b:Comp B) :
+  Comp_eq (_ <-$ a; b) b.
+Admitted. (* TODO: does FCF have something like this? *)
 
 Section Language.
-  Context {base_type : Set} {interp_base_type:base_type->Set}.
+  Context {base_type : Set}
+          {interp_base_type:base_type->nat->Set}
+          {eqdec_base_type : forall {t eta}, EqDec (interp_base_type t eta)}.
 
   Inductive type := Type_base (t:base_type) | Type_arrow (dom:type) (cod:type).
   Global Coercion Type_base : base_type >-> type.
-  Fixpoint interp_type (t:type) : Set :=
+  Fixpoint interp_type (t:type) (eta:nat) : Set :=
     match t with
-    | Type_base t => interp_base_type t
-    | Type_arrow dom cod => interp_type dom -> interp_type cod
+    | Type_base t => interp_base_type t eta
+    | Type_arrow dom cod => interp_type dom eta -> interp_type cod eta
     end.
+  Delimit Scope term_scope with term.
+  Bind Scope term_scope with type.
+  Notation "A -> B" := (Type_arrow A B) : term_scope.
 
-  Context {message list_message rand : base_type}.
+  Context {bool message list_message rand : base_type}
+          {true false:forall eta, interp_type bool eta}.
+  (* we would need a dependently typed map data structure for dependently typed randomness *)
 
   (* A term is parametrized by its type, which can either be one of the base_types *)
   (* listed above, or an arrow type consisting of multiple interpreted base_types. *)
   Inductive term : type -> Type :=
-  | Term_const {t} (_: nat -> interp_type t) : term t
-  | Term_random (_:nat) : term rand
+  | Term_const {t} (_:forall eta, interp_type t eta) : term t
+  | Term_random (idx:positive) : term rand
   | Term_adversarial (_:term list_message) : term message
   | Term_app {dom cod} (_:term (Type_arrow dom cod)) (_:term dom) : term cod.
-
-  (* the first natural number that is not a valid randomness index *)
-  Fixpoint rand_end {t:type} (e:term t) : nat :=
-    match e with
-    | Term_random n => S n
-    | Term_app f x => max (rand_end f) (rand_end x)
-    | _ => 0
-    end.
-
-  Context (interp_random : nat -> interp_type rand).
-  Context (interp_adversarial : interp_type list_message -> interp_type message).
-  Fixpoint interp_term
-           {t} (e:term t) (eta : nat) : interp_type t :=
-    match e with
-    | Term_const c => c eta
-    | Term_random n => interp_random n
-    | Term_adversarial ctx => interp_adversarial (interp_term ctx eta)
-    | Term_app f x => (interp_term f eta) (interp_term x eta)
-    end.
-End Language.
-
-Arguments type : clear implicits.
-Arguments interp_type {_} _ _.
-Arguments term {_} _ _ _ _ _.
-Arguments rand_end [_ _ _ _ _ _] _.
-
-Section CompInterp.
-  (* We explicitly distinguish between randomness and a message type *)
-  Inductive base_type := BaseType_bool | BaseType_message | BaseType_list_message | BaseType_rand.
-  Definition interp_base_type t :=
-    match t with
-    | BaseType_bool => bool
-    | BaseType_message => list bool
-    | BaseType_list_message => list (list bool)
-    | BaseType_rand => list bool
-    end.
-
-  Let term := (term interp_base_type BaseType_message BaseType_list_message BaseType_rand).
-  
-  (* TODO: we aither need to only allow computing base types OR require all types to be finite *)
-  Global Instance interp_eqdec : forall {t}, EqDec (interp_type interp_base_type t).
-  Admitted.
-
-  (* different protocols may use different amounts of randomness at the same security level. this is an awkward and boring parameter *)
-
-  (* TODO: each term rnd should have it's own size as a function of eta, then the max would be adding together bits that everything needs (this will eliminate multiplication) *)
-  Context (rand_size : nat -> nat).
-
-  Section WithAdversary.
-    (* the adversary is split into three parts for no particular reason. It first decides how much randomness it will need, then interacts with the protocol (repeated calls to [adverary] with all messages up to now as input), and then tries to claim victory ([distinguisher]). There is no explicit sharing of state between these procedures, but all of them get the same random inputs in the security game. The handling of state is a major difference between FCF [OracleComp] and this framework *)
-    Context (evil_rand_tape_len : nat -> nat).
-    Context (adversary:nat -> list bool -> list (list bool) -> list bool).
-    Context (distinguisher: forall {t}, nat -> list bool -> interp_type interp_base_type t -> bool).
-
-    Definition comp_interp_term_fixed (good_rand_tape evil_rand_tape:list bool) eta {t} (e:term t) :=
-      let interp_random (n:nat) : interp_type interp_base_type (Type_base BaseType_rand)
-          := List.firstn (rand_size eta) (List.skipn (n * rand_size eta) good_rand_tape) in
-      let interp_adversarial : interp_type interp_base_type (Type_arrow (Type_base BaseType_list_message) (Type_base BaseType_message))
-          := adversary eta evil_rand_tape in
-      interp_term interp_random interp_adversarial e eta.
-
-    Definition comp_interp_term eta {t:type base_type} (e:term t)  : Comp (interp_type interp_base_type t) :=
-      good_rand_tape' <-$ {0,1}^(rand_end e * rand_size eta);
-        evil_rand_tape' <-$ {0,1}^(evil_rand_tape_len eta);
-        let good_rand_tape := Vector.to_list good_rand_tape' in
-        let evil_rand_tape := Vector.to_list evil_rand_tape' in
-        ret (comp_interp_term_fixed good_rand_tape evil_rand_tape eta e).
-            
-    Definition universal_security_game eta {t:type base_type} (e:term t) : Comp bool :=
-      good_rand_tape' <-$ {0,1}^(rand_end e * rand_size eta);
-        evil_rand_tape' <-$ {0,1}^(evil_rand_tape_len eta);
-        let good_rand_tape := Vector.to_list good_rand_tape' in
-        let evil_rand_tape := Vector.to_list evil_rand_tape' in
-        let out := comp_interp_term_fixed good_rand_tape evil_rand_tape eta e in
-        ret (distinguisher _ eta evil_rand_tape out).
-
-  End WithAdversary.
-
-  Definition indist {t:type base_type} (a b:term t) : Prop :=  forall l adv dst,
-      (* TODO: insert bounds on coputational complexity of [adv] and [dst] here *)
-      let game eta e := universal_security_game l adv dst eta e in
-      negligible (fun eta => | Pr[game eta a] -  Pr[game eta b] | ).
-  Global Instance Reflexive_indist {t} : Reflexive (@indist t).
-  Proof.
-    cbv [Reflexive indist]; setoid_rewrite ratDistance_same; eauto using negligible_0.
-  Qed.
-
-  Global Instance Symmetric_indist {t} : Symmetric (@indist t).
-  Proof.
-    cbv [Symmetric indist]; intros; setoid_rewrite ratDistance_comm; eauto.
-  Qed.
-
-  Delimit Scope term_scope with term.
-
-  Notation "A -> B" := (Type_arrow A B) : term_scope.
+  Bind Scope term_scope with term.
   Notation "A @ B" := (Term_app A B) (at level 99) : term_scope.
-
   Notation "'rnd' n" := (Term_random n) (at level 35) : term_scope.
   Notation "'const' c" := (Term_const c) (at level 35) : term_scope.
 
-  Notation s_message := (Type_base BaseType_message).
-  Notation s_rand := (Type_base BaseType_rand).
-  Notation s_bool := (Type_base BaseType_bool).
+  Fixpoint randomness_indices {t:type} (e:term t) : PositiveSet.t :=
+    match e with
+    | Term_random idx => PositiveSet.singleton idx
+    | Term_app f x => PositiveSet.union (randomness_indices f) (randomness_indices x)
+    | _ => PositiveSet.empty
+    end.
+  Global Instance randomness_map_eq_dec {eta} : EqDec (PositiveMap.t (interp_type rand eta)). Admitted.
+  Context (len_rand : forall eta:nat, nat)
+          (cast_rand : forall eta, Bvector (len_rand eta) -> interp_type rand eta).
+  Definition generate_randomness idxs (eta:nat)
+    : Comp (PositiveMap.t (interp_type rand eta))
+    := PositiveSet.fold (fun i rndC => (
+                             rnds' <-$ rndC;
+                               ri <-$ {0,1}^(len_rand eta);
+                               ret (PositiveMap.add i (cast_rand eta ri) rnds')
+                           )%comp)
+                        idxs
+                        (ret (PositiveMap.empty _)).
 
-  Section Eqwhp.
-    Definition s_true : nat -> interp_type interp_base_type s_bool := fun _ => true.
-    Definition s_eqb : nat -> interp_type interp_base_type (s_bool -> s_bool -> s_bool)%term := fun _ => eqb.
+  Context (unreachable:forall {i}, Bvector (len_rand i)).
+  Global Instance EqDec_interp_type : forall t eta, EqDec (interp_type t eta). Admitted. (* TODO: functional extensionality? *)
+  Fixpoint interp_term_fixed {t} (e:term t) (eta : nat)
+           (adv: interp_type list_message eta -> interp_type message eta)
+           (rands: PositiveMap.t (interp_type rand eta))
+    : interp_type t eta :=
+    match e with
+    | Term_const c => c eta
+    | Term_random i => match PositiveMap.find i rands with Some r => r | _ => cast_rand eta (unreachable _) end
+    | Term_adversarial ctx => adv (interp_term_fixed ctx eta adv rands)
+    | Term_app f x => (interp_term_fixed f eta adv rands) (interp_term_fixed x eta adv rands)
+    end.
+  Definition interp_term {t} (e:term t) (eta:nat)
+             (adv: interp_type list_message eta -> interp_type message eta)
+    : Comp (interp_type t eta)
+    := rands <-$ generate_randomness (randomness_indices e) eta; ret (interp_term_fixed e eta adv rands).
 
-    Definition eqwhp (b0 b1 : forall _ : nat, interp_type interp_base_type s_bool) : Prop :=
-      indist (const s_eqb @ (const b0) @ (const b1))%term (const s_true)%term.
+  Section Security.
+    (* the adversary is split into three parts for no particular reason. It first decides how much randomness it will need, then interacts with the protocol (repeated calls to [adverary] with all messages up to now as input), and then tries to claim victory ([distinguisher]). There is no explicit sharing of state between these procedures, but all of them get the same random inputs in the security game. The handling of state is a major difference between FCF [OracleComp] and this framework *)
+    Definition universal_security_game 
+               (evil_rand_tape_len: forall eta:nat, nat)
+               (adversary:forall (eta:nat) (rand:Bvector (evil_rand_tape_len eta)), interp_type list_message eta -> interp_type message eta)
+               (distinguisher: forall {t} (eta:nat) (rand:Bvector (evil_rand_tape_len eta)), interp_type t eta -> Datatypes.bool)
+               (eta:nat) {t:type} (e:term t) : Comp Datatypes.bool :=
+      evil_rand_tape <-$ {0,1}^(evil_rand_tape_len eta);
+        out <-$ interp_term e eta (adversary eta (evil_rand_tape));
+        ret (distinguisher eta evil_rand_tape out).
 
-    Global Instance Reflexive_eqwhp : Reflexive eqwhp.
+    Definition indist {t:type} (a b:term t) : Prop :=  forall adl adv dst,
+        (* TODO: insert bounds on coputational complexity of [adv] and [dst] here *)
+        let game eta e := universal_security_game adl adv dst eta e in
+        negligible (fun eta => | Pr[game eta a] -  Pr[game eta b] | ).
+
+    Global Instance Reflexive_indist {t} : Reflexive (@indist t).
     Proof.
-      simpl.
-      intros.
-      cbv [Reflexive indist universal_security_game eqwhp s_eqb rand_end].
-      intros.
-      pose proof negligible_const_num 1.
-      apply eq_impl_negligible.
-      intros eta.
-      apply Comp_eq_bool.
-      fcf_well_formed.
-      fcf_well_formed.
-      rewrite Nat.max_0_l.
-      fcf_skip.
-      fcf_skip.
-      apply evalDist_ret_eq.
-      apply f_equal.
-      cbv [comp_interp_term_fixed interp_term s_true].
-      apply eqb_refl.
+      cbv [Reflexive indist]; setoid_rewrite ratDistance_same; eauto using negligible_0.
     Qed.
 
-    Global Instance Symmetric_eqwhp : Symmetric eqwhp.
+    Global Instance Symmetric_indist {t} : Symmetric (@indist t).
     Proof.
-      simpl.
-      intros.
-      cbv [Symmetric indist universal_security_game eqwhp s_eqb rand_end].
-      intros.
-      pose proof negligible_const_num 1.
-      apply eq_impl_negligible.
-      intros eta.
-      apply Comp_eq_bool.
-      fcf_well_formed.
-      fcf_well_formed.
-      rewrite Nat.max_0_l.
-      fcf_skip.
-      fcf_skip.
-      apply evalDist_ret_eq.
-      apply f_equal.
-      cbv [comp_interp_term_fixed interp_term s_true].
+      cbv [Symmetric indist]; intros; setoid_rewrite ratDistance_comm; eauto.
+    Qed.
+  End Security.
 
+  Definition whp (e:term bool) := indist e (const true).
+
+  Section Equality.
+    Definition const_eqb t : term (t -> t -> bool) :=
+      @Term_const
+        (Type_arrow t (Type_arrow t (Type_base bool)))
+        (fun eta x1 x2 => if eqb x1 x2 then true eta else false eta).
+    Definition eqwhp {t:type} (e1 e2:term t) : Prop := whp (const_eqb t @ e1 @ e2)%term.
+
+    Global Instance Reflexive_eqwhp {t} : Reflexive (@eqwhp t).
+    Proof.
+      cbv [Reflexive indist universal_security_game eqwhp whp interp_term]; intros.
+      apply eq_impl_negligible; intro eta.
+      eapply Proper_Bind; [reflexivity|]; intros ? ? ?; subst.
+      eapply Proper_Bind; [|intros ? ? ?; subst; reflexivity]. 
+      simpl interp_term_fixed.
+      etransitivity.
+      { eapply Proper_Bind; [reflexivity|]; intros ? ? ?; subst.
+        (* TODO: why can't we do this earlier (under binders) using setoid_rewrite? *)
+        rewrite eqb_refl.
+        instantiate (1:=fun _ => ret true eta); cbv beta.
+        reflexivity. }
+      rewrite 2Bind_unused.
+      reflexivity.
+    Qed.
+  End Equality.
+
+  Section LateInterp.
+    Fixpoint interp_term_late
+             {t} (e:term t) (eta : nat)
+             (adv: interp_type list_message eta -> interp_type message eta)
+             (fixed_rand: PositiveMap.t (interp_type rand eta))
+    : Comp (interp_type t eta) :=
+      match e with
+      | Term_const c => ret (c eta)
+      | Term_random i =>
+        match PositiveMap.find i fixed_rand with
+        | Some r => ret r
+        | _ => r <-$ {0,1}^(len_rand eta); ret (cast_rand eta r)
+        end
+      | Term_adversarial ctx =>
+        ctx <-$ interp_term_late ctx eta adv fixed_rand; ret (adv ctx)
+      | Term_app f x => 
+        common_rand <-$ generate_randomness (PositiveSet.inter (randomness_indices x) (randomness_indices f)) eta;
+          rands <- PositiveMapProperties.update common_rand fixed_rand;
+          x <-$ interp_term_late x eta adv rands;
+          f <-$ interp_term_late f eta adv rands;
+          ret (f x)
+      end.
+    Lemma interp_term_late_correct {t} (e:term t) eta adv :
+      Comp_eq (interp_term_late e eta adv (PositiveMap.empty _)) (interp_term e eta adv).
+      (* this form is not strong enough for induction *)
     Admitted.
-  End Eqwhp.
+  End LateInterp.
 
-  (* randomness -> key *)
-  Context (KeyGen : nat -> interp_type interp_base_type (s_rand -> s_message)%term).
-  (* key -> randomness -> plaintext -> ciphertext *)
-  Context (Encrypt : nat -> interp_type interp_base_type (s_message -> s_rand -> s_message -> s_message)%term).
-  (* key -> ciphertext -> plaintext *)
-  Context (Decrypt : nat -> interp_type interp_base_type (s_message -> (s_message -> s_message))%term).
-
-  Context (admissible_A1: pred_oc_fam).
-  Context (admissible_A2: pred_oc_func_2_fam).
-
-  Fixpoint disjoint A (xl yl : list A) :=
-    match xl with
-    | nil => True
-    | x :: xl => ~ In x yl /\ disjoint A xl yl
-    end.
-
-  Fixpoint rands_in {t} (x : term t) : list nat :=
-    match x with
-      | Term_random n => n :: nil
-      | Term_app func arg => rands_in func ++ rands_in arg
-      | _ => nil
-    end.
-
-  (* Lemma rand_split : forall {dom cod} (func : term (Type_arrow dom cod)) (arg : term dom), *)
-  (*     exists (lfunc larg lshare : list nat), *)
-  (*       NoDup lfunc -> *)
-  (*       NoDup larg -> *)
-  (*       NoDup lshare -> *)
-  (*       disjoint lfunc larg -> *)
-  (*       disjoint larg lshare -> *)
-  (*       disjoint lfunc lshare -> *)
-  (*       length lfunc + length larg + length lshare = rand_end (Term_app func arg) -> *)
-
-
-  (*       Comp_eq  (r <-$ {0, 1} ^ rand_end (Term_app func arg); *)
-  (*                ) *)
-
-
-
-
-    (* Term_app {dom cod} (_:term (Type_arrow dom cod)) (_:term dom) : term cod *)
-    (* If functions take different randomness as direct arguments, you can split up into + *)
-    (* forall (t : term), partition into three sets of randomness, used in a, used in b, used in a + b *)
-(* exists (a, b, c : list nat), (a b c are disjoint, elements are unique, sum of lengths = rand_end t), comp_eq ({0, 1} ^ rand_end t) ( *)
-
-  (* TODO: split good_rand_tape into two separate binds *)
-  (* TODO: p0, p1 are arbitrary terms that cannot include (rnd r) or (rnd n0) *)
-  Lemma indist_encrypt
-  (p0 p1 : forall _ : nat, interp_type interp_base_type (s_message))
-  (r n0 n1: nat)
-  (HNoDup:NoDup (r::n0::n1::nil))
-  : indist (const Encrypt @ (const KeyGen @ (rnd r)) @ (rnd n0) @ (const p0))%term
-           (const Encrypt @ (const KeyGen @ (rnd r)) @ (rnd n1) @ (const p1))%term.
+  Lemma indist_rand (x y:positive) : indist (rnd x) (rnd y).
   Proof.
-    cbv [indist universal_security_game comp_interp_term interp_term].
-    intros.
-                                                                                                        (* coq positive map, randomness is map from index to slot *)
-    (* forall (t : term), if two subterms are disjoint, you can partition into two randomnesses *)
-
-    (* , comp_eq ({0, 1} ^ rand_end t) (you can partition rand_end t into n sections/ loop from 0 to n and sum to get the distribution) *)
-    (* [ecut] ? *)
-    evar (T1:Type); evar (e1:T1); subst T1.
-    evar (T2:Type); evar (e2:T2); subst T2.
-    evar (T3:Type); evar (e3:T3); subst T3.
-    evar (T4:Type); evar (e4:T4); subst T4.
-    evar (T5:Type); evar (e5:T5); subst T5.
-    evar (T6:Type); evar (e6:T6); subst T6.
-    evar (T7:Type); evar (e7:T7); subst T7.
-    evar (T8:Type); evar (e8:T8); subst T8.
-    evar (eIND:@IND_CPA_SecretKey e1 e2 e3 e4 e5 e6 e7 e8); clearbody eIND.
-    subst e1 e2 e3 e4 e5 e6 e7 e8.
-    cbv[IND_CPA_SecretKey IND_CPA_SecretKey_Advantage] in eIND.
-    (* 
-    eapply TwoWorlds_equiv'.
-    admit.
-    admit.
-    cbv [StandardDef_G'].
-    cbv [IND_CPA_SecretKey_G] in eIND.
-    cbv [EncryptOracle] in eIND.
-     *) 
-
-    (* map from randomness index to option randomness *)
-    (* rewrite interpretation function to push randomness down as low as possible by keeping around map with either already generated or not yet generated randomness *)
-    (* prove that two interpretation functions are equal *)
-    (* Lemma rand_split : forall adv evil_rand_tape' eta *)
-    (*                      {dom cod} (func : term (Type_arrow dom cod)) (arg : term dom), *)
-    (*   exists (lfunc larg lshare : list nat), *)
-    (*     NoDup lfunc -> *)
-    (*     NoDup larg -> *)
-    (*     NoDup lshare -> *)
-    (*     disjoint lfunc larg -> *)
-    (*     disjoint larg lshare -> *)
-    (*     disjoint lfunc lshare -> *)
-    (*     length lfunc + length larg + length lshare = rand_end (Term_app func arg) -> *)
-
-
-    (*     Comp_eq (good_rand_tape <-$ {0, 1} ^ rand_end (Term_app func arg); *)
-    (*                ret (comp_interp_term_fixed adv *)
-    (*                                            (Vector.to_list good_rand_tape') *)
-    (*                                            (Vector.to_list evil_rand_tape') *)
-    (*                                            eta *)
-    (*                                            cod *)
-    (*                                            (Term_app func arg))) *)
-    (*             (rshare <-$ {0, 1} ^ length lshare; *)
-    (*                rarg <-$ {0, 1} ^ length larg; *)
-    (*                comp_interp_term_fixed adv *)
-
-
-    (*                arg' <-$ comp_interp_term_fixed adv *)
-    (*                                            (Vector.to_list good_rand_tape') *)
-    (*                                            (Vector.to_list evil_rand_tape') *)
-
-
-
-    (* (* split it, move good_rand_tape generation down as much as possible *) *)
-    (* (* group good_rand_tape + encrypt, good_rand_tape + keygen *) *)
-    (* (* instantiate (e6 := (thing that generates comp, bind in goal with good_rand_tape)) *) *)
-    (* (* A1 -- generate constant *) *)
-    (* (* A2 - everything else *) *)
-
-
-    (* instantiate (e7 := fun _ _ _ _ => True). *)
-    (* instantiate (e8 := fun _ _ _ _ _ _ => True). *)
-    (* cbv beta in eIND. *)
-
-    (* eapply IND_CPA_SecretKey_equiv in eIND. *)
-
-    (* eapply TwoWorlds_equiv in eIND. *)
-
-  (* generalize (random_size eta) as D; intro D. *)
-    Admitted.
-
-(** proving soundness of symbolic axioms *)
-  End CompInterp.
-
-Section SymbolicProof.
-  Context {base_type : Set} {interp_base_type : base_type -> Set}.
-  Local Coercion type_base (t:base_type) : type base_type := Type_base t.
-  Context {message list_message rand bool : base_type}.
-
-  Local Notation term := (term interp_base_type message list_message rand).
-  Context (indist : forall {t : type base_type}, term t -> term t -> Prop). Arguments indist {_} _ _.
-
-  Context (if_then_else : forall {t}, term (Type_arrow bool (Type_arrow t (Type_arrow t t)))). Arguments if_then_else {_}.
-  Context (indist_rand: forall x y, indist (Term_random x) (Term_random y)).
-  Context (indist_if_then_else_irrelevant_l : forall t (x y:term t),
-              indist x y -> forall b:term bool, indist (Term_app (Term_app (Term_app if_then_else b) x) y) x).
-
-  Lemma indist_if_then_else_rand_l (b:term bool) (x y:nat) :
-    indist (Term_app (Term_app (Term_app if_then_else b) (Term_random x)) (Term_random y)) (Term_random x).
-  Proof. exact (indist_if_then_else_irrelevant_l _ _ _ (indist_rand x y) _). Qed.
-End SymbolicProof.
-
-Definition if_then_else {t : type base_type}
-  : interp_type interp_base_type (Type_arrow (type_base BaseType_bool) (Type_arrow t (Type_arrow t t)))
-  := fun (b : bool) (x y : interp_type interp_base_type t) => if b then x else y.
-
-Lemma indist_rand random_size (x y : nat) : indist random_size (Term_random x) (Term_random y).
-Proof.
-  cbv [rand_end indist universal_security_game comp_interp_term interp_term]. (* to monadic probability notation *)
-  intros.
-  pose proof negligible_const_num 1.
-  apply eq_impl_negligible.
-  intros eta.
-  apply Comp_eq_bool.
-  fcf_well_formed.
-  fcf_well_formed.
-  dist_swap_l.
-  dist_swap_r.
-  fcf_skip.
-
-  assert (Pr [c <-$ (d <-$ (a <-$ { 0 , 1 }^ x * random_size eta + random_size eta; ret (splitVector (x * random_size eta) (random_size eta) a)); ret snd d);
-              ret dst (Type_base BaseType_rand) eta (Vector.to_list x0) (Vector.to_list c) ] ==
-          Pr [c <-$ (d <-$ (a <-$ { 0 , 1 }^ y * random_size eta + random_size eta; ret (splitVector (y * random_size eta) (random_size eta) a)); ret snd d);
-              ret dst (Type_base BaseType_rand) eta (Vector.to_list x0) (Vector.to_list c) ] ).
-  {
-    fcf_skip.
-    match goal with |- evalDist ?C1 ?x == evalDist ?C2 ?x => generalize x; change (Comp_eq C1 C2) end.
-    setoid_rewrite Rnd_split_eq.
-    apply Comp_eq_evalDist.
-    {
-      fcf_well_formed.
-    }
-    {
-      fcf_well_formed.
-    }
-    {
-      intros.
-      fcf_inline_first.
-      fcf_at fcf_inline fcf_left 1%nat.
-      fcf_at fcf_inline fcf_right 1%nat.
-      fcf_swap fcf_left.
-      fcf_swap fcf_right.
-      fcf_skip.
-      fcf_at fcf_ret fcf_left 1%nat.
-      fcf_at fcf_ret fcf_right 1%nat.
-      cbv [snd].
-      fcf_irr_l.
-      {
-        fcf_well_formed.
-      }
-      fcf_irr_r.
-      {
-        fcf_well_formed.
-      }
-    }
-  }
-  etransitivity.
-  etransitivity.
-  2: apply H1.
-
-  fcf_inline_first.
-  replace (S x * random_size eta)%nat with (x * random_size eta + random_size eta)%nat by ring.
-  fcf_skip.
-  fcf_simp.
-  apply evalDist_ret_eq.
-  repeat f_equal.
-  cbv [comp_interp_term_fixed interp_term].
-  rewrite list_vector_split.
-  eapply firstn_ge_all.
-  rewrite to_list_length.
-  auto.
-
-  fcf_inline_first.
-  replace (S y * random_size eta)%nat with (y * random_size eta + random_size eta)%nat by ring.
-  fcf_skip.
-  fcf_simp.
-  apply evalDist_ret_eq.
-  repeat f_equal.
-  cbv [comp_interp_term_fixed interp_term].
-  rewrite list_vector_split.
-  symmetry.
-  eapply firstn_ge_all.
-  rewrite to_list_length.
-  auto.
-Qed.
+    cbv [indist]; intros.
+    apply eq_impl_negligible; cbv [pointwise_relation]; intros eta.
+    cbv [universal_security_game].
+    (* setoid_rewrite <-interp_term_late_correct. WHY does it not work? *)
+    eapply Proper_Bind; [reflexivity|]; intros ? ? ?; subst.
+    setoid_rewrite <-interp_term_late_correct.
+    simpl interp_term_late.
+    rewrite 2PositiveMap.gempty.
+    reflexivity.
+  Qed.
+End Language.
+Arguments type _ : clear implicits.
